Add more types of abstract states

src/high/abstract_state.v
@@ -3,6 +3,9 @@ From stdpp Require Export countable.
 From self Require Import extra.
 
 Class AbstractState ST `{Countable ST} := {
+  (* NOTE: The definition makes use of [relation2] as using [relation] (or
+  anything that refers to it such as [SqSubsetEq] causes universe issues due to
+  Iris. *)
   abs_state_relation : relation2 ST;
   abs_state_preorder :> PreOrder abs_state_relation;
 }.
