src/high/abstract_state_instances.v
@@ -1,28 +1,19 @@
 From stdpp Require Export countable.
 
 From self Require Import extra.
+From self.algebra Require Import view.
 From self.high Require Import abstract_state.
 
 (** We define abstract state for some common types. *)
 
 (* Abstract state for booleans. *)
-Instance sqsubseteq_bool : SqSubsetEq bool := λ b1 b2,
-    if b1 then b2 = true else True.
 
-Instance subseteq_bool_preorder : PreOrder (⊑@{bool}).
-Proof. split; repeat intros [|]; done. Qed.
+Program Instance bool_abstract_state : AbstractState bool :=
+  { abs_state_relation b1 b2 := if b1 then b2 = true else True }.
+Next Obligation. split; repeat intros [|]; done. Qed.
 
-Instance bool_abstract_state : AbstractState bool.
-Proof. esplit; apply _. Defined.
-
-(* Abstract state for natural numbers. *)
-Instance sqsubseteq_nat : SqSubsetEq nat := λ v w, v ≤ w.
-
-Instance subseteq_nat_preorder : PreOrder (⊑@{nat}).
-Proof. apply _. Qed.
-
-Instance nat_abstract_state : AbstractState nat.
-Proof. esplit; apply _. Defined.
+Program Instance nat_abstract_state : AbstractState nat :=
+  { abs_state_relation := (≤) }.
 
 Lemma subseteq_nat_le (n m : nat) : n ⊑ m = (n ≤ m).
 Proof. done. Qed.
@@ -32,11 +23,6 @@ Record singl (A : Type) := mk_singl { get_singl : A }.
 Arguments mk_singl {A}.
 Arguments get_singl {A}.
 
-Instance sqsubseteq_singl A : SqSubsetEq (singl A) := λ u1 u2, True.
-
-Instance subseteq_singl_preorder A : PreOrder (⊑@{singl A}).
-Proof. done. Qed.
-
 Instance singl_eqdecision A `{EqDecision A} : EqDecision (singl A).
 Proof. 
   unfold EqDecision in *. unfold Decision in *. decide equality.
@@ -44,7 +30,7 @@ Qed.
 
 Instance singl_countable A `{Countable A} : Countable (singl A).
 Proof.
-  refine (inj_countable' get_singl mk_singl _).
+  apply (inj_countable' get_singl mk_singl).
   intros [x]. reflexivity.
 Qed.
 
@@ -53,15 +39,10 @@ Proof. esplit; apply _. Defined.
 
 (* Abstract state for unit. *)
 
-Instance sqsubseteq_unit : SqSubsetEq unit := λ u1 u2, True.
-
-Instance subseteq_unit_preorder : PreOrder (⊑@{unit}).
-Proof. done. Qed.
-
 Instance unit_abstract_state : AbstractState unit.
 Proof. esplit; apply _. Defined.
 
-(** * discreteState abstract state. *)
+(** Discrete abstract state (only reflexivity). *)
 
 Record discreteState A := mk_discrete { get_discrete : A }.
 
@@ -83,12 +64,60 @@ Section discrete_abstract_state.
     |}.
   Next Obligation. intros ??[?]. rewrite decode_encode. done. Qed.
 
-  Global Instance discrete_sqsubseteq : SqSubsetEq (discreteState A) := λ a1 a2, a1 = a2.
-
-  Global Instance subseteq_discrete_preorder : PreOrder (⊑@{discreteState A}).
-  Proof. apply _. Qed.
-
   Global Instance discrete_abstract_state `{Countable A} : AbstractState (discreteState A).
   Proof. esplit; apply _. Defined.
 
 End discrete_abstract_state.
+
+(** Numbered abstract state. *)
+
+Inductive numbered (A : Type) := mk_numbered : nat → A → numbered A.
+
+Arguments mk_numbered {A} n a.
+
+Section numbered_abstract_state.
+  Context `{Countable A}.
+
+  Global Instance numbered_discreteeq : EqDecision (numbered A).
+  Proof.
+    unfold EqDecision in *. unfold Decision in *.
+    decide equality. decide equality.
+  Qed.
+
+  Global Instance numbered_countable : Countable (numbered A).
+  Proof.
+    apply (inj_countable' (λ '(mk_numbered n a), (n, a))
+                          (λ '(n, a), mk_numbered n a)).
+    intros [??]. reflexivity.
+  Qed.
+
+  Global Program Instance numbered_abstract_state : AbstractState (numbered A) :=
+    {
+      abs_state_relation '(mk_numbered n1 a1) '(mk_numbered n2 a2) :=
+        n1 < n2 ∨ (n1 = n2 ∧ a1 = a2)
+    }.
+  Next Obligation.
+    constructor.
+    - intros [??]. right. done.
+    - intros [??] [??] [??] [?|[??]] [?|[??]]; try (left; naive_solver lia).
+      right. split; congruence.
+  Qed.
+
+  Global Instance numbered_antisym : AntiSymm (=) (⊑@{numbered A}).
+  Proof. intros [??] [??] [?|[??]] [?|[??]]; lia || congruence. Qed.
+
+  Lemma numbered_le n1 n2 a1 a2 :
+    n1 < n2 →
+    mk_numbered n1 a1 ⊑ mk_numbered n2 a2.
+  Proof. intros ?. left. done. Qed.
+
+End numbered_abstract_state.
+
+(** Product abstract state. *)
+
+Section prod_abstract_state.
+
+  Global Instance prod_abstract_state `{AbstractState A} `{AbstractState B} :
+    AbstractState (A * B) := {}.
+
+End prod_abstract_state.
